Generate inversion lemmas using idt.

theories/lang_oadt/inversion.v
@@ -1,4 +1,5 @@
 (** Typing and kinding inversion lemmas. *)
+From oadt Require Import idt.
 From oadt Require Import lang_oadt.base.
 From oadt Require Import lang_oadt.syntax.
 From oadt Require Import lang_oadt.semantics.
@@ -7,7 +8,6 @@ From oadt Require Import lang_oadt.infrastructure.
 From oadt Require Import lang_oadt.equivalence.
 
 Import syntax.notations.
-Import semantics.notations.
 Import typing.notations.
 Import equivalence.notations.
 
@@ -16,510 +16,52 @@ Implicit Types (b : bool) (x X y Y : atom) (L : aset).
 #[local]
 Coercion EFVar : atom >-> expr.
 
-Section inversion.
-
-Context (Σ : gctx).
-
-#[local]
-Set Default Proof Using "Type".
-
 (** * Kind inversion  *)
-Tactic Notation "kind_inv_solver" "by" tactic3(tac) :=
-  match goal with
-  | |- _ ⊢ ?τ :: _ -> _ => remember τ
-  end;
-  induction 1; subst; simp_hyps; simplify_eq;
-  tac.
 
-Ltac kind_inv_solver :=
-  kind_inv_solver by (repeat esplit; eauto;
-                      lattice_naive_solver by eauto using top_inv, join_ub_r).
-
-Lemma kind_inv_pi Γ l τ1 τ2 κ :
-  Γ ⊢ Π:{l}τ1, τ2 :: κ ->
-  κ = <{ *@M }> /\
-  exists L κ1 κ2,
-    (∀ x, x ∉ L → (<[x:=(l, τ1)]> Γ) ⊢ τ2^x :: κ2) /\
-    Γ ⊢ τ1 :: κ1.
-Proof.
-  kind_inv_solver.
-Qed.
-
-Lemma kind_inv_bool Γ κ :
-  Γ ⊢ 𝔹 :: κ -> <{ *@P }> ⊑ κ.
-Proof.
-  kind_inv_solver.
-Qed.
-
-Lemma kind_inv_prod Γ τ1 τ2 κ :
-  Γ ⊢ τ1 * τ2 :: κ ->
-  exists κ',
-    Γ ⊢ τ1 :: κ' /\
-    Γ ⊢ τ2 :: κ' /\
-    <{ κ' }> ⊑ κ.
-Proof.
-  kind_inv_solver.
-Qed.
-
-Lemma kind_inv_sum Γ τ1 τ2 κ :
-  Γ ⊢ τ1 + τ2 :: κ ->
-  <{ *@P }> ⊑ κ /\
-  exists κ',
-    Γ ⊢ τ1 :: κ' /\
-    Γ ⊢ τ2 :: κ'.
-Proof.
-  kind_inv_solver.
-Qed.
-
-Lemma kind_inv_osum Γ τ1 τ2 κ :
-  Γ ⊢ τ1 ~+ τ2 :: κ ->
-  <{ *@O }> ⊑ κ /\
-  Γ ⊢ τ1 :: *@O /\
-  Γ ⊢ τ2 :: *@O.
-Proof.
-  kind_inv_solver.
-Qed.
-
-Lemma kind_inv_gvar Γ X κ :
-  Γ ⊢ gvar X :: κ ->
-  <{ *@P }> ⊑ κ /\ exists τ, Σ !! X = Some (DADT τ).
-Proof.
-  kind_inv_solver.
-Qed.
-
-Lemma kind_inv_tapp Γ X e κ :
-  Γ ⊢ X@e :: κ ->
-  <{ *@O }> ⊑ κ /\
-  exists τ e',
-    Σ !! X = Some (DOADT τ e') /\
-    Γ ⊢ e :{⊥} τ.
-Proof.
-  kind_inv_solver.
-Qed.
-
-Lemma kind_inv_ite Γ l e0 τ1 τ2 κ :
-  Γ ⊢ if{l} e0 then τ1 else τ2 :: κ ->
-  <{ *@O }> ⊑ κ /\
-  l = LPub /\
-  Γ ⊢ e0 :{⊥} 𝔹 /\
-  Γ ⊢ τ1 :: *@O /\
-  Γ ⊢ τ2 :: *@O.
-Proof.
-  kind_inv_solver.
-Qed.
-
-Lemma kind_inv_let Γ e τ κ :
-  Γ ⊢ let e in τ :: κ ->
-  <{ *@O }> ⊑ κ /\
-  exists τ' L,
-    Γ ⊢ e :{⊥} τ' /\
-    (forall x, x ∉ L -> <[x:=(⊥, τ')]> Γ ⊢ τ^x :: *@O).
-Proof.
-  kind_inv_solver.
-Qed.
-
-Lemma kind_inv_case Γ l e0 τ1 τ2 κ :
-  Γ ⊢ case{l} e0 of τ1 | τ2 :: κ ->
-  <{ *@O }> ⊑ κ /\
-  l = LPub /\
-  exists τ1' τ2' L1 L2,
-    Γ ⊢ e0 :{⊥} τ1' + τ2' /\
-    (forall x, x ∉ L1 -> <[x:=(⊥, τ1')]> Γ ⊢ τ1^x :: *@O) /\
-    (forall x, x ∉ L2 -> <[x:=(⊥, τ2')]> Γ ⊢ τ2^x :: *@O).
-Proof.
-  kind_inv_solver.
-Qed.
-
-Lemma kind_inv_app Γ e1 e2 κ :
-  Γ ⊢ e1 e2 :: κ -> False.
-Proof.
-  kind_inv_solver.
-Qed.
-
-Lemma kind_inv_oite Γ e0 e1 e2 κ :
-  Γ ⊢ ~if e0 then e1 else e2 :: κ -> False.
-Proof.
-  kind_inv_solver.
-Qed.
-
-Lemma kind_inv_mux Γ e0 e1 e2 κ :
-  Γ ⊢ mux e0 e1 e2 :: κ -> False.
-Proof.
-  kind_inv_solver.
-Qed.
-
-Lemma kind_inv_sec Γ e κ :
-  Γ ⊢ s𝔹 e :: κ -> False.
-Proof.
-  kind_inv_solver.
-Qed.
-
-Lemma kind_inv_pair Γ e1 e2 κ :
-  Γ ⊢ (e1, e2) :: κ -> False.
-Proof.
-  kind_inv_solver.
-Qed.
-
-Lemma kind_inv_proj Γ b e κ :
-  Γ ⊢ π@b e :: κ -> False.
-Proof.
-  kind_inv_solver.
-Qed.
-
-Lemma kind_inv_inj Γ l b τ e κ :
-  Γ ⊢ inj{l}@b<τ> e :: κ -> False.
-Proof.
-  kind_inv_solver.
-Qed.
-
-Lemma kind_inv_ocase Γ e0 e1 e2 κ :
-  Γ ⊢ ~case e0 of e1 | e2 :: κ -> False.
-Proof.
-  kind_inv_solver.
-Qed.
-
-Lemma kind_inv_fold Γ X e κ :
-  Γ ⊢ fold<X> e :: κ -> False.
-Proof.
-  kind_inv_solver.
-Qed.
-
-Lemma kind_inv_unfold Γ X e κ :
-  Γ ⊢ unfold<X> e :: κ -> False.
-Proof.
-  kind_inv_solver.
-Qed.
-
-Lemma kind_inv_abs Γ l τ e κ :
-  Γ ⊢ \:{l}τ => e :: κ -> False.
-Proof.
-  kind_inv_solver.
-Qed.
-
-Lemma kind_inv_tape Γ e κ :
-  Γ ⊢ tape e :: κ -> False.
-Proof.
-  kind_inv_solver.
-Qed.
-
-(** * Type inversion *)
-Tactic Notation "type_inv_solver" "by" tactic3(tac) :=
-  match goal with
-  | |- _ ⊢ ?e : _ -> _ => remember e
-  end;
-  induction 1; subst; simp_hyps; simplify_eq;
-  tac.
-
-Ltac type_inv_solver :=
-  type_inv_solver by (repeat (eauto; esplit);
-                      try first [ goal_is (_ ≡ _); equiv_naive_solver
-                                | try select kind (fun k => clear dependent k);
-                                  lattice_naive_solver
-                                    by eauto using (top_inv (A:=bool)) ]).
-
-Lemma type_inv_prod Γ l τ1 τ2 τ :
-  Γ ⊢ τ1 * τ2 :{l} τ -> False.
-Proof.
-  type_inv_solver.
-Qed.
-
-Lemma type_inv_sum Γ l l' τ1 τ2 τ :
-  Γ ⊢ τ1 +{l} τ2 :{l'} τ -> False.
-Proof.
-  type_inv_solver.
-Qed.
-
-Lemma type_inv_tapp Γ l X e τ :
-  Γ ⊢ X@e :{l} τ -> False.
-Proof.
-  type_inv_solver.
-Qed.
-
-(** From now on the proofs rely on the well-formedness of global context. *)
-Context (Hwf : gctx_wf Σ).
-
-#[local]
-Set Default Proof Using "Hwf".
-
-Lemma type_inv_unit Γ l τ :
-  Γ ⊢ () :{l} τ ->
-  τ ≡ <{ 𝟙 }>.
-Proof.
-  type_inv_solver.
-Qed.
-
-Lemma type_inv_lit Γ l b τ :
-  Γ ⊢ lit b :{l} τ ->
-  τ ≡ <{ 𝔹 }>.
-Proof.
-  type_inv_solver.
-Qed.
-
-Lemma type_inv_abs Γ l1 l2 e τ2 τ :
-  Γ ⊢ \:{l2}τ2 => e :{l1} τ ->
-  exists l1' τ1 κ L,
-    Γ ⊢ τ2 :: κ /\
-    (forall x, x ∉ L -> <[x:=(l2, τ2)]> Γ ⊢ e^x :{l1'} τ1^x) /\
-    l1' ⊑ l1 /\
-    τ ≡ <{ Π:{l2}τ2, τ1 }>.
-Proof.
-  type_inv_solver.
-Qed.
-
-Lemma type_inv_gvar Γ l x τ :
-  Γ ⊢ gvar x :{l} τ ->
-  exists l' τ' e,
-    Σ !! x = Some (DFun (l', τ') e) /\
-    l' ⊑ l /\
-    τ ≡ τ'.
-Proof.
-  type_inv_solver.
-Qed.
-
-Lemma type_inv_pair Γ l e1 e2 τ :
-  Γ ⊢ (e1, e2) :{l} τ ->
-  exists l1 l2 τ1 τ2,
-    Γ ⊢ e1 :{l1} τ1 /\
-    Γ ⊢ e2 :{l2} τ2 /\
-    l1 ⊔ l2 ⊑ l /\
-    τ ≡ <{ τ1 * τ2 }>.
-Proof.
-  type_inv_solver.
-Qed.
-
-Lemma type_inv_inj Γ l b e τ' τ :
-  Γ ⊢ inj@b<τ'> e :{l} τ ->
-  exists l' τ1 τ2 κ,
-    τ' = <{ τ1 + τ2 }> /\
-    Γ ⊢ τ1 + τ2 :: κ /\
-    Γ ⊢ e :{l'} ite b τ1 τ2 /\
-    l' ⊑ l /\
-    τ ≡ <{ τ1 + τ2 }>.
-Proof.
-  type_inv_solver.
-Qed.
-
-Lemma type_inv_oinj Γ l b e τ' τ :
-  Γ ⊢ ~inj@b<τ'> e :{l} τ ->
-  exists τ1 τ2,
-    τ' = <{ τ1 ~+ τ2 }> /\
-    Γ ⊢ τ1 ~+ τ2 :: *@O /\
-    Γ ⊢ e :{⊥} ite b τ1 τ2 /\
-    τ ≡ <{ τ1 ~+ τ2 }>.
-Proof.
-  type_inv_solver.
-Qed.
-
-Lemma type_inv_fold Γ l X e τ :
-  Γ ⊢ fold<X> e :{l} τ ->
-  exists l' τ',
-    Γ ⊢ e :{l'} τ' /\
-    Σ !! X = Some (DADT τ') /\
-    l' ⊑ l /\
-    τ ≡ <{ gvar X }>.
-Proof.
-  type_inv_solver.
-Qed.
-
-Lemma type_inv_boxedlit Γ l b τ :
-  Γ ⊢ [b] :{l} τ ->
-  τ ≡ <{ ~𝔹 }>.
-Proof.
-  type_inv_solver.
-Qed.
-
-Lemma type_inv_boxedinj Γ l b v ω τ :
-  Γ ⊢ [inj@b<ω> v] :{l} τ ->
-  exists ω1 ω2,
-    ω = <{ ω1 ~+ ω2 }> /\
-    ovalty <{ [inj@b<ω> v] }> ω /\
-    τ ≡ <{ ω1 ~+ ω2 }>.
-Proof.
-  type_inv_solver by hauto lq: on ctrs: ovalty inv: ovalty
-                           solve: equiv_naive_solver.
-Qed.
-
-Lemma type_inv_case Γ l e0 e1 e2 τ :
-  Γ ⊢ case e0 of e1 | e2 :{l} τ ->
-  exists l0 l1 l2 τ1 τ2 τ' κ L1 L2,
-    Γ ⊢ τ'^e0 :: κ /\
-    Γ ⊢ e0 :{l0} τ1 + τ2 /\
-    (forall x, x ∉ L1 -> <[x:=(l0, τ1)]> Γ ⊢ e1^x :{l1} τ'^(inl<τ1 + τ2> x)) /\
-    (forall x, x ∉ L2 -> <[x:=(l0, τ2)]> Γ ⊢ e2^x :{l2} τ'^(inr<τ1 + τ2> x)) /\
-    l0 ⊔ l1 ⊔ l2 ⊑ l /\
-    τ ≡ <{ τ'^e0 }>.
-Proof.
-  type_inv_solver.
-
-  all : intros;
-    lazymatch goal with
-    | H : _; _ ⊢ ?τ :: _ |- _ =>
-      rewrite (open_lc_intro τ) by eauto using kinding_lc
-    end; eauto; equiv_naive_solver.
-Qed.
-
-Lemma type_inv_ocase Γ l e0 e1 e2 τ :
-  Γ ⊢ ~case e0 of e1 | e2 :{l} τ ->
-  exists l1 l2 τ1 τ2 τ' κ L1 L2,
-    Γ ⊢ τ' :: κ /\
-    Γ ⊢ e0 :{⊥} τ1 ~+ τ2 /\
-    (forall x, x ∉ L1 -> <[x:=(⊥, τ1)]> Γ ⊢ e1^x :{l1} τ') /\
-    (forall x, x ∉ L2 -> <[x:=(⊥, τ2)]> Γ ⊢ e2^x :{l2} τ') /\
-    τ ≡ τ'.
-Proof.
-  type_inv_solver.
-Qed.
-
-Lemma type_inv_case_ Γ l l' e0 e1 e2 τ :
-  Γ ⊢ case{l} e0 of e1 | e2 :{l'} τ ->
-  exists l0 l1 l2 τ1 τ2 τ' κ L1 L2,
-    Γ ⊢ τ' :: κ /\
-    Γ ⊢ e0 :{l0} τ1 +{l} τ2 /\
-    (forall x, x ∉ L1 -> exists τ', <[x:=(l0, τ1)]> Γ ⊢ e1^x :{l1} τ') /\
-    (forall x, x ∉ L2 -> exists τ', <[x:=(l0, τ2)]> Γ ⊢ e2^x :{l2} τ') /\
-    τ ≡ τ'.
-Proof.
-  type_inv_solver.
-Qed.
-
-Lemma type_inv_app Γ l1 e1 e2 τ :
-  Γ ⊢ e1 e2 :{l1} τ ->
-  exists l1' l2 τ1 τ2,
-    Γ ⊢ e1 :{l1'} Π:{l2}τ2, τ1 /\
-    Γ ⊢ e2 :{l2} τ2 /\
-    l1' ⊑ l1 /\
-    τ ≡ <{ τ1^e2 }>.
-Proof.
-  type_inv_solver.
-Qed.
-
-Lemma type_inv_let Γ l e1 e2 τ :
-  Γ ⊢ let e1 in e2 :{l} τ ->
-  exists l1 l2 τ1 τ2 L,
-    Γ ⊢ e1 :{l1} τ1 /\
-    (forall x, x ∉ L -> <[x:=(l1, τ1)]> Γ ⊢ e2^x :{l2} τ2^x) /\
-    l1 ⊔ l2 ⊑ l /\
-    τ ≡ <{ τ2^e1 }>.
-Proof.
-  type_inv_solver.
-Qed.
-
-Lemma type_inv_sec Γ l e τ :
-  Γ ⊢ s𝔹 e :{l} τ ->
-  exists l',
-    Γ ⊢ e :{l'} 𝔹 /\
-    l' ⊑ l /\
-    τ ≡ <{ ~𝔹 }>.
-Proof.
-  type_inv_solver.
-Qed.
-
-Lemma type_inv_ite Γ l e0 e1 e2 τ :
-  Γ ⊢ if e0 then e1 else e2 :{l} τ ->
-  exists l0 l1 l2 τ',
-    Γ ⊢ e0 :{l0} 𝔹 /\
-    Γ ⊢ e1 :{l1} τ'^(lit true) /\
-    Γ ⊢ e2 :{l2} τ'^(lit false) /\
-    l0 ⊔ l1 ⊔ l2 ⊑ l /\
-    τ ≡ <{ τ'^e0 }>.
-Proof.
-  type_inv_solver.
-
-  all :
-    lazymatch goal with
-    | H : _; _ ⊢ _ : ?τ |- _ =>
-      rewrite (open_lc_intro τ) by eauto using typing_type_lc
-    end; eauto; try equiv_naive_solver.
-Qed.
-
-Lemma type_inv_oite Γ l e0 e1 e2 τ :
-  Γ ⊢ ~if e0 then e1 else e2 :{l} τ ->
-  exists l1 l2 τ' κ,
-    Γ ⊢ e0 :{⊥} ~𝔹 /\
-    Γ ⊢ e1 :{l1} τ' /\
-    Γ ⊢ e2 :{l2} τ' /\
-    Γ ⊢ τ' :: κ /\
-    l = ⊤ /\
-    τ ≡ τ'.
-Proof.
-  type_inv_solver.
-Qed.
-
-Lemma type_inv_mux Γ l e0 e1 e2 τ :
-  Γ ⊢ mux e0 e1 e2 :{l} τ ->
-  exists τ',
-    Γ ⊢ e0 :{⊥} ~𝔹 /\
-    Γ ⊢ e1 :{⊥} τ' /\
-    Γ ⊢ e2 :{⊥} τ' /\
-    Γ ⊢ τ' :: *@O /\
-    τ ≡ τ'.
-Proof.
-  type_inv_solver.
-Qed.
-
-Lemma type_inv_proj Γ l b e τ :
-  Γ ⊢ π@b e :{l} τ ->
-  exists l' τ1 τ2,
-    Γ ⊢ e :{l'} τ1 * τ2 /\
-    l' ⊑ l /\
-    τ ≡ <{ ite b τ1 τ2 }>.
-Proof.
-  type_inv_solver.
-Qed.
-
-Lemma type_inv_unfold Γ l X e τ :
-  Γ ⊢ unfold<X> e :{l} τ ->
-  exists l' τ',
-    Σ !! X = Some (DADT τ') /\
-    Γ ⊢ e :{l'} gvar X /\
-    l' ⊑ l /\
-    τ ≡ τ'.
-Proof.
-  type_inv_solver.
-Qed.
-
-Lemma type_inv_tape Γ l e τ :
-  Γ ⊢ tape e :{l} τ ->
-  exists l' τ',
-    Γ ⊢ e :{l'} τ' /\
-    Γ ⊢ τ' :: *@O /\
-    τ ≡ τ'.
-Proof.
-  type_inv_solver.
-Qed.
-
-End inversion.
-
-(** * Tactics *)
-
-Tactic Notation "kind_inv" hyp(H) "by" tactic3(tac) :=
-  lazymatch type of H with
-  | _; _ ⊢ Π:{_}_, _ :: _ => tac kind_inv_pi
-  | _; _ ⊢ 𝔹 :: _ => tac kind_inv_bool
-  | _; _ ⊢ _@_ :: _ => tac kind_inv_tapp
-  | _; _ ⊢ let _ in _ :: _ => tac kind_inv_let
-  | _; _ ⊢ _ * _ :: _ => tac kind_inv_prod
-  | _; _ ⊢ _ + _ :: _ => tac kind_inv_sum
-  | _; _ ⊢ _ ~+ _ :: _ => tac kind_inv_osum
-  | _; _ ⊢ gvar _ :: _ => tac kind_inv_gvar
-  | _; _ ⊢ _ _ :: _ => apply kind_inv_app in H; elim H
-  | _; _ ⊢ ~if _ then _ else _ :: _ => apply kind_inv_oite in H; elim H
-  | _; _ ⊢ if{_} _ then _ else _ :: _ => tac kind_inv_ite
-  | _; _ ⊢ ~case _ of _ | _ :: _ => apply kind_inv_ocase in H; elim H
-  | _; _ ⊢ case{_} _ of _ | _ :: _ => tac kind_inv_case
-  | _; _ ⊢ s𝔹 _ :: _ => apply kind_inv_sec in H; elim H
-  | _; _ ⊢ (_, _) :: _ => apply kind_inv_pair in H; elim H
-  | _; _ ⊢ π@_ _ :: _ => apply kind_inv_proj in H; elim H
-  | _; _ ⊢ inj{_}@_<_> _ :: _ => apply kind_inv_inj in H; elim H
-  | _; _ ⊢ fold<_> _ :: _ => apply kind_inv_fold in H; elim H
-  | _; _ ⊢ unfold<_> _ :: _ => apply kind_inv_unfold in H; elim H
-  | _; _ ⊢ \:{_}_ => _ :: _ => apply kind_inv_abs in H; elim H
-  | _; _ ⊢ mux _ _ _ :: _ => apply kind_inv_mux in H; elim H
-  | _; _ ⊢ tape _ :: _ => apply kind_inv_tape in H; elim H
+Ltac tsf_kinding ctor R :=
+  lazymatch ctor with
+  | KSub => tsf_skip
+  | _ =>
+      let H := fresh in
+      pose proof ctor as H;
+      repeat
+        lazymatch type of H with
+        | forall e : ?T, _ =>
+            refine (forall e : T, _ : Prop); specialize (H e)
+        | ?Σ; ?Γ ⊢ ?τ :: ?κ =>
+            let κ' := fresh "κ'" in
+            refine (forall κ', _ : Prop);
+            lazymatch κ with
+            | <{ *@M }> => refine (κ' = <{ *@M }> -> _ : Prop)
+            | <{ *@A }> => idtac
+            | <{ ?κ1 ⊔ ?κ2 }> => refine (κ1 ⊑ κ' -> κ2 ⊑ κ' -> _ : Prop)
+            | _ => refine (κ ⊑ κ' -> _ : Prop)
+            end;
+            refine (R Σ Γ τ κ' : Prop)
+        end
   end.
 
+MetaCoq Run (tsf_ind_gen_from
+               kinding "kinding_inv"
+               (ltac:(tsf_ctors kinding (append "I") tsf_kinding))).
+
+Lemma kinding_inv_complete Σ Γ τ κ :
+  Σ; Γ ⊢ τ :: κ ->
+  kinding_inv Σ Γ τ κ.
+Proof.
+  induction 1; eauto using kinding_inv, join_ub_l, join_ub_r.
+
+  select (kinding_inv _ _ _ _) (fun H => destruct H);
+    econstructor; subst; eauto using top_inv with lattice_naive_solver.
+Qed.
+
 Tactic Notation "kind_inv" hyp(H) :=
-  kind_inv H by (fun lem => apply lem in H; try simp_hyp H).
+  lazymatch type of H with
+  | _ ⊢ ?τ :: _ =>
+      head_constructor τ;
+      apply kinding_inv_complete in H;
+      sinvert H
+  end.
 
 Tactic Notation "kind_inv" :=
   do_hyps (fun H => try kind_inv H).
@@ -527,40 +69,111 @@ Tactic Notation "kind_inv" :=
 Tactic Notation "kind_inv" "*" :=
   do_hyps (fun H => try dup_hyp H (fun H => kind_inv H)).
 
-Tactic Notation "type_inv" hyp(H) "by" tactic3(tac) :=
-  lazymatch type of H with
-  | _; _ ⊢ () : _ => tac type_inv_unit
-  | _; _ ⊢ lit _ : _ => tac type_inv_lit
-  | _; _ ⊢ gvar _ : _ => tac type_inv_gvar
-  | _; _ ⊢ \:{_}_ => _ : _ => tac type_inv_abs
-  | _; _ ⊢ _ _ : _ => tac type_inv_app
-  | _; _ ⊢ let _ in _ : _ => tac type_inv_let
-  | _; _ ⊢ (_, _) : _ => tac type_inv_pair
-  | _; _ ⊢ s𝔹 _ : _ => tac type_inv_sec
-  | _; _ ⊢ π@_ _ : _ => tac type_inv_proj
-  | _; _ ⊢ ~inj@_<_> _ : _ => tac type_inv_oinj
-  | _; _ ⊢ inj@_<_> _ : _ => tac type_inv_inj
-  | _; _ ⊢ ~if _ then _ else _ : _ => tac type_inv_oite
-  | _; _ ⊢ if _ then _ else _ : _ => tac type_inv_ite
-  | _; _ ⊢ ~case _ of _ | _ : _ => tac type_inv_ocase
-  | _; _ ⊢ case _ of _ | _ : _ => tac type_inv_case
-  | _; _ ⊢ case{_} _ of _ | _ : _ => tac type_inv_case_
-  | _; _ ⊢ fold<_> _ : _ => tac type_inv_fold
-  | _; _ ⊢ unfold<_> _ : _ => tac type_inv_unfold
-  | _; _ ⊢ mux _ _ _ : _ => tac type_inv_mux
-  | _; _ ⊢ tape _ : _ => tac type_inv_tape
-  | _; _ ⊢ [_] : _ => tac type_inv_boxedlit
-  | _; _ ⊢ [inj@_<_> _] : _ => tac type_inv_boxedinj
-  | _; _ ⊢ _ * _ : _ => apply type_inv_prod in H; elim H
-  | _; _ ⊢ _ +{_} _ : _ => apply type_inv_sum in H; elim H
-  | _; _ ⊢ _@_ : _ => apply type_inv_tapp in H; elim H
+
+(** * Type inversion *)
+
+Module kernel.
+
+Section fix_gctx.
+
+Context (Σ : gctx).
+
+(** [TIte] and [TCase] require special rules. *)
+Inductive typing_inv : tctx -> expr -> bool -> expr -> Prop :=
+| ITIte Γ l0 l1 l2 l e0 e1 e2 τ :
+    Γ ⊢ e0 :{l0} 𝔹 ->
+    Γ ⊢ e1 :{l1} τ^(lit true) ->
+    Γ ⊢ e2 :{l2} τ^(lit false) ->
+    l = l0 ⊔ l1 ⊔ l2 ->
+    forall l' τ',
+      l ⊑ l' ->
+      τ' ≡ <{ τ^e0 }> ->
+      typing_inv Γ <{ if e0 then e1 else e2 }> l' τ'
+| ITCase Γ l0 l1 l2 l e0 e1 e2 τ1 τ2 τ κ L1 L2 :
+    Γ ⊢ e0 :{l0} τ1 + τ2 ->
+    (forall x, x ∉ L1 -> Σ; <[x:=(l0, τ1)]>Γ ⊢ e1^x :{l1} τ^(inl<τ1 + τ2> x)) ->
+    (forall x, x ∉ L2 -> Σ; <[x:=(l0, τ2)]>Γ ⊢ e2^x :{l2} τ^(inr<τ1 + τ2> x)) ->
+    Γ ⊢ τ^e0 :: κ ->
+    l = l0 ⊔ l1 ⊔ l2 ->
+    forall l' τ',
+      l ⊑ l' ->
+      τ' ≡ <{ τ^e0 }> ->
+      typing_inv Γ <{ case e0 of e1 | e2 }> l' τ'
+.
+
+End fix_gctx.
+
+End kernel.
+
+Ltac tsf_typing ctor R :=
+  lazymatch ctor with
+  (* Remove the cases about [TIte] and [TCase]. *)
+  | TIteNoDep => tsf_skip
+  | TCaseNoDep => tsf_skip
+  | TIte => tsf_skip
+  | TCase => tsf_skip
+  | TConv => tsf_skip
+  | _ =>
+      let H := fresh in
+      pose proof ctor as H;
+      repeat
+        lazymatch type of H with
+        | forall e : ?T, _ =>
+            refine (forall e : T, _ : Prop); specialize (H e)
+        | ?Σ; ?Γ ⊢ ?e :{?l} ?τ =>
+            let l' := fresh "l'" in
+            let τ' := fresh "τ'" in
+            refine (forall (l' : llabel) (τ' : expr), _ : Prop);
+            lazymatch l with
+            | ⊤ => refine (l' = ⊤ -> _ : Prop)
+            | ⊥ => idtac
+            | _ => refine (l ⊑ l' -> _ : Prop)
+            end;
+            refine (Σ ⊢ τ' ≡ τ -> R Σ Γ e l' τ' : Prop)
+        end
   end.
 
+MetaCoq Run (tsf_ind_gen_from
+               typing "typing_inv"
+               (ltac:(tsf_ctors typing (append "I") tsf_typing) ++
+                ltac:(tsf_ctors_id kernel.typing_inv))).
+
+
+Lemma typing_inv_complete Σ Γ e l τ :
+  gctx_wf Σ ->
+  Σ; Γ ⊢ e :{l} τ ->
+  typing_inv Σ Γ e l τ.
+Proof.
+  intros Hwf.
+  induction 1; eauto using typing_inv with equiv_naive_solver.
+
+  (* TIte *)
+  - econstructor; eauto;
+    lazymatch goal with
+    | H : _ ⊢ _ : ?τ |- _ =>
+        rewrite (open_lc_intro τ) by eauto using typing_type_lc
+    end; eauto with equiv_naive_solver.
+
+  (* TCase *)
+  - econstructor; eauto; intros;
+    lazymatch goal with
+    | H : _ ⊢ ?τ :: _ |- _ =>
+        rewrite (open_lc_intro τ) by eauto using kinding_lc
+    end; eauto with equiv_naive_solver.
+
+  (* TConv *)
+  - select (typing_inv _ _ _ _ _) (fun H => sinvert H);
+    econstructor; subst;
+    eauto using (top_inv (A:=bool)) with equiv_naive_solver lattice_naive_solver.
+Qed.
+
 Tactic Notation "type_inv" hyp(H) :=
-  type_inv H by (fun lem => apply lem in H; try simp_hyp H);
-  try lazymatch goal with
-      | |- gctx_wf _ => assumption
-      end.
+  lazymatch type of H with
+  | _ ⊢ ?e : _ =>
+      head_constructor e;
+      apply typing_inv_complete in H;
+      [ sinvert H; try ovalty_inv | assumption ]
+  end.
 
 Tactic Notation "type_inv" :=
   do_hyps (fun H => try type_inv H).
